Verity/Macro/Translate.lean
@@ -1,6 +1,7 @@
 import Lean
 import Compiler.Modules.ERC20
 import Compiler.Modules.Calls
+import Compiler.Modules.Oracle
 import Compiler.Modules.Precompiles
 import Compiler.Selectors
 import Compiler.CompilationModel.InternalNaming
@@ -1331,15 +1332,25 @@ private partial def translateDoElem
                               let targetExpr ← translatePureExprWithTypes fields constDecls immutableDecls params locals target
                               let argExprs ← argTerms.mapM
                                 (translatePureExprWithTypes fields constDecls immutableDecls params locals)
-                              let isStaticTerm ← if ext.isView then `(true) else `(false)
+                              let stmt ←
+                                if ext.isView then
+                                  `(Compiler.CompilationModel.Stmt.ecm
+                                      (Compiler.Modules.Oracle.typedReadWordSummaryModule
+                                        $(strTerm varName)
+                                        $(strTerm ext.name)
+                                        $(natTerm selector)
+                                        $(natTerm argExprs.size))
+                                      [ $targetExpr, $[$argExprs],* ])
+                                else
+                                  `(Compiler.CompilationModel.Stmt.ecm
+                                      (Compiler.Modules.Calls.withReturnModule
+                                        $(strTerm varName)
+                                        $(natTerm selector)
+                                        $(natTerm argExprs.size)
+                                        false)
+                                      [ $targetExpr, $[$argExprs],* ])
                               pure
-                                (#[(← `(Compiler.CompilationModel.Stmt.ecm
-                                        (Compiler.Modules.Calls.withReturnModule
-                                          $(strTerm varName)
-                                          $(natTerm selector)
-                                          $(natTerm argExprs.size)
-                                          $isStaticTerm)
-                                        [ $targetExpr, $[$argExprs],* ]))],
+                                (#[stmt],
                                   locals.push (mkTypedLocal varName retTy),
                                   mutableLocals)
                           | some (_, _, _, none, _) =>
